backwards direction

theories/SeparationLogic/Reductions/FSAT_to_MSPSAT.v
@@ -6,9 +6,13 @@ From Undecidability.SeparationLogic Require Import min_seplogic.
 From Undecidability Require Import Shared.ListAutomation.
 Import ListAutomationNotations.
 
+From Undecidability.Shared Require Import Dec.
+From Equations Require Import Equations.
+
+
 (** encoding function **)
 
-Fixpoint encode {b : falsity_flag} (phi : form) : msp_form :=
+Fixpoint encode {ff : falsity_flag} (phi : form) : msp_form :=
   match phi with
   | falsity => mbot
   | atom _ v => let x := match Vector.hd v with var x => x | func f _ => match f with end end in
@@ -24,6 +28,166 @@ Fixpoint encode {b : falsity_flag} (phi : form) : msp_form :=
 
 Definition encode' (phi : form) : msp_form :=
   mimp (mex (mpointer (Some 0) None None)) (encode phi).
+
+
+
+(** backward direction **)
+
+Lemma pointers_disc :
+  eq_dec (nat * (val * val)).
+Proof.
+  exact _.
+Qed.
+
+Lemma map_hd X Y n (f : X -> Y) (v : Vector.t X (S n)) :
+  Vector.hd (Vector.map f v) = f (Vector.hd v).
+Proof.
+  dependent elimination v. reflexivity.
+Qed.
+
+Lemma map_tl X Y n (f : X -> Y) (v : Vector.t X (S n)) :
+  Vector.tl (Vector.map f v) = Vector.map f (Vector.tl v).
+Proof.
+  dependent elimination v. reflexivity.
+Qed.
+
+Lemma in_hd X n (v : Vector.t X (S n)) :
+  Vector.In (Vector.hd v) v.
+Proof.
+  dependent elimination v. constructor.
+Qed.
+
+Lemma in_hd_tl X n (v : Vector.t X (S (S n))) :
+  Vector.In (Vector.hd (Vector.tl v)) v.
+Proof.
+  dependent elimination v. constructor. dependent elimination t. constructor.
+Qed.
+
+Definition FV_term (t : term) : nat :=
+  match t with
+  | $n => n
+  | func f v => match f with end
+  end.
+
+Fixpoint FV {ff : falsity_flag} (phi : form) : list nat :=
+  match phi with
+  | falsity => nil
+  | atom _ v => map FV_term (Vector.to_list v)
+  | bin b phi psi => (FV phi) ++ (FV psi)
+  | quant q phi => map pred (filter (fun n : nat => if n then false else true) (FV phi))
+  end.
+
+Lemma to_list_iff X n (v : Vector.t X n) x :
+  x el Vector.to_list v <-> Vector.In x v.
+Proof.
+  induction v; cbn; split.
+Admitted.
+
+Section Backwards.
+
+  Definition defined (h : heap) l :=
+    if Dec ((l, (None, None)) el h) then True else False.
+
+  Lemma defined_iff h l :
+    defined h l <-> (l, (None, None)) el h.
+  Proof.
+    unfold defined. split; destruct Dec; tauto.
+  Defined.
+
+  Definition dom (h : heap) : Type :=
+    { l | defined h l }.
+
+  Definition loc2dom {h : heap} {l} :
+    (l, (None, None)) el h -> dom h.
+  Proof.
+    intros H. exists l. now apply defined_iff.
+  Defined.
+
+  Lemma loc2dom_eq h l (H H' : (l, (None, None)) el h) :
+    loc2dom H = loc2dom H'.
+  Proof.
+    unfold loc2dom. cbn. f_equal. destruct Dec; trivial. contradiction.
+  Qed.
+
+  Definition env (s : stack) (h : heap) (d : dom h) :
+    nat -> dom h.
+  Proof.
+    intros n. destruct (s n) as [l |].
+    - decide ((l, (None, None)) el h).
+      + exact (loc2dom i).
+      + exact d.
+    - exact d.
+  Defined.
+
+  Instance model h :
+    interp (dom h).
+  Proof.
+    split.
+    - intros [].
+    - intros [] v. exact (exists l, (l, (Some (proj1_sig (Vector.hd v)), Some (proj1_sig (Vector.hd (Vector.tl v))))) el h).
+  Defined.
+
+  Lemma update_stack_cons s h l d (H : (l, (None, None)) el h) x :
+    env (update_stack s (Some l)) h d x = (loc2dom H .: env s h d) x.
+  Proof.
+    destruct x as [|x]; try reflexivity.
+    cbn. destruct Dec; try tauto. apply loc2dom_eq.
+  Qed.
+
+  Lemma update_stack_cons' s h d0 d x :
+    (d .: env s h d0) x = env (update_stack s (Some (proj1_sig d))) h d0 x.
+  Proof.
+    destruct d, x as [|x]; try reflexivity. cbn. destruct Dec.
+    - unfold loc2dom. f_equal. admit.
+    - contradict n. now apply defined_iff.
+  Admitted.
+
+  Lemma reduction_backwards (s : stack) (h : heap) (d0 : dom h) phi :
+    (forall x, x el FV phi -> exists l, s x = Some l /\ (l, (None, None)) el h) -> env s h d0 ⊨ phi <-> msp_sat s h (encode phi).
+  Proof.
+    induction phi in s |- *; try destruct P; try destruct b0; try destruct q; cbn; intros HV.
+    - tauto.
+    - rewrite map_tl, !map_hd. destruct (Vector.hd t) as [x|[]] eqn : Hx.
+      destruct (Vector.hd (Vector.tl t)) as [y|[]] eqn : Hy. cbn. split.
+      + intros [l Hl].
+        destruct (HV x) as (l1 & H1 & H2).
+        { apply in_map_iff. exists (Vector.hd t). split; try now rewrite Hx. apply to_list_iff, in_hd. }
+        destruct (HV y) as (l2 & H3 & H4).
+        { apply in_map_iff. exists (Vector.hd (Vector.tl t)). split; try now rewrite Hy. apply to_list_iff, in_hd_tl. }
+        unfold env in Hl. rewrite H1, H3 in Hl. do 2 destruct Dec; try tauto. cbn in Hl. repeat split.
+        * exists (Some l), l. split; trivial. now rewrite H1, H3.
+        * now exists l1.
+        * now exists l2.
+     + intros [[v[l[-> Hl]]][[l1[H1 H2]][l2[H3 H4]]]]. exists l. unfold env. rewrite H1, H3.
+       do 2 destruct Dec; try tauto. cbn. now rewrite <- H1, <- H3.
+  - rewrite IHphi1, IHphi2; try tauto. all: intros x Hx; apply HV; apply in_app_iff; auto.
+  - rewrite IHphi1, IHphi2; try tauto. all: intros x Hx; apply HV; apply in_app_iff; auto.
+  - rewrite IHphi1, IHphi2; try tauto. all: intros x Hx; apply HV; apply in_app_iff; auto.
+  - split; intros H.
+    + intros [l|] [l'[H1 H2]]; try discriminate. injection H1. intros <-. apply IHphi.
+      * intros [|x] Hx; try now exists l. apply HV. apply in_map_iff. exists (S x). split; trivial. now apply in_filter_iff.
+      * eapply sat_ext; try apply (H (loc2dom H2)). apply update_stack_cons.
+    + intros [l Hl]. eapply sat_ext, IHphi, H.
+      * apply update_stack_cons'.
+      * cbn. assert (Hl' : (l, (None, None)) el h) by now apply defined_iff.
+        intros [|x] Hx; try now exists l. apply HV. apply in_map_iff. exists (S x). split; trivial. now apply in_filter_iff.
+      * cbn. exists l. split; trivial. now apply defined_iff.
+  - split; intros H.
+    + destruct H as [[l Hl] H]. assert (Hl' : (l, (None, None)) el h) by now apply defined_iff.
+      exists (Some l). split; try now exists l. apply IHphi.
+      * intros [|x] Hx; try now exists l. apply HV. apply in_map_iff. exists (S x). split; trivial. now apply in_filter_iff.
+      * eapply sat_ext; try apply H. intros x. now rewrite update_stack_cons'.
+    + destruct H as [[l|][[l'[H1 H2]] H]]; try discriminate. injection H1. intros <-.
+      exists (loc2dom H2). eapply sat_ext, IHphi, H.
+      * intros x. now erewrite update_stack_cons.
+      * intros [|x] Hx; try now exists l. apply HV. apply in_map_iff. exists (S x). split; trivial. now apply in_filter_iff.
+  Qed.
+
+End Backwards. 
+
+
+
+(** reduction theorem **)
 
 Require Import Undecidability.Synthetic.Definitions.
 
